polishing equiv

HL/Equiv.lean
@@ -19,33 +19,22 @@ file := some "Equiv"
 open scoped HasEval MyGetElem Com
 ```
 
-:::dev "Sati (satiscugcat)"
-  At this point, the Rocq file provides instructions about using a new directory,
-  making sure the project is set up properly, and also instructions about how to
-  deal with the exercises. I am assuming these things are being moved to Intro.lean?
-  I am excluding them for now.
-:::
+# Behavioral Equivalence
 
-```lean
-open scoped HasEval MyGetElem
-```
-
-# Behavioral Equivaleence
 ::::full
+In {ref "Slang"}[an earlier chapter], we investigated the correctness of a very
+simple program transformation: the `optimize0plus` function.  The
+programming language we were considering was the first version of
+the language of arithmetic expressions - with no variables - so
+in that setting it was very easy to define what it means for a
+program transformation to be correct: it should always yield a
+program that evaluates to the same number as the original.
 
-  In an earlier chapter, we investigated the correctness of a very
-  simple program transformation: the `optimize0plus` function.  The
-  programming language we were considering was the first version of
-  the language of arithmetic expressions -- with no variables -- so
-  in that setting it was very easy to define what it means for a
-  program transformation to be correct: it should always yield a
-  program that evaluates to the same number as the original.
-
-  To talk about the correctness of program transformations for the
-  full Imp language -- in particular, assignment -- we need to
-  consider the role of mutable state and develop a more
-  sophisticated notion of correctness, which we'll call _behavioral
-  equivalence_.
+To talk about the correctness of program transformations for the
+full Imp language - in particular, assignment - we need to
+consider the role of mutable state and develop a more
+sophisticated notion of correctness, which we'll call _behavioral
+equivalence_.
 ::::
 
 ::::full
@@ -68,17 +57,36 @@ def Aexp.Equiv (a₁ a₂ : Aexp) : Prop :=
   ∀ (st : State),
     a₁.eval st = a₂.eval st
 
-theorem Aexp.equiv_def {a₁ a₂ : Aexp} :
-    a₁.Equiv a₂ ↔ ∀ (st : State), a₁.eval st = a₂.eval st := by rfl
-```
-
-```lean
 def Bexp.Equiv (b₁ b₂ : Bexp) : Prop :=
   ∀ (st : State),
     b₁.eval st = b₂.eval st
+```
 
+We'll also define a notation for `Equiv`:
+
+```lean
+class Equiv (α : Type) where
+  equiv : α → α → Prop
+
+infix:70 " ≃ " => Equiv.equiv -- you can type `≃` as \equiv
+
+instance : Equiv Aexp where
+  equiv := Aexp.Equiv
+
+instance : Equiv Bexp where
+  equiv := Bexp.Equiv
+
+@[simp]
+theorem Aexp.equiv_notation {a₁ a₂ : Aexp} : a₁.Equiv a₂ ↔ a₁ ≃ a₂ := by rfl
+@[simp]
+theorem Aexp.equiv_def {a₁ a₂ : Aexp} :
+    a₁ ≃ a₂ ↔ ∀ (st : State), a₁.eval st = a₂.eval st := by rfl
+
+@[simp]
+theorem Bexp.equiv_notation {b₁ b₂ : Bexp} : b₁.Equiv b₂ ↔ b₁ ≃ b₂ := by rfl
+@[simp]
 theorem Bexp.equiv_def {b₁ b₂ : Bexp} :
-    b₁.Equiv b₂ ↔ ∀ (st : State), b₁.eval st = b₂.eval st := by rfl
+    b₁ ≃ b₂ ↔ ∀ (st : State), b₁.eval st = b₂.eval st := by rfl
 ```
 
 ::::full
@@ -87,45 +95,41 @@ and boolean expressions.
 ::::
 
 ```lean
-example : Aexp.Equiv
-    (aexp { X - X })
-    (aexp { 0 }) := by
-  rw [Aexp.equiv_def]
-  intro st
-  simp
+example : aexp { X - X } ≃ aexp { 0 } := by simp
 ```
 
 
 ```lean
-example : Bexp.Equiv
-    (bexp { X - X = 0 })
-    (bexp { true }) := by
-  rw [Bexp.equiv_def]
-  intro st
-  simp
+example : bexp { X - X = 0 } ≃ bexp { true } := by simp
 ```
 
 ::::full
-  For commands, the situation is a little more subtle.  We
-  can't simply say "two commands are behaviorally equivalent if they
-  evaluate to the same ending state whenever they are started in the
-  same initial state," because some commands, when run in some
-  starting states, don't terminate in any final state at all!
+For commands, the situation is a little more subtle.  We
+can't simply say "two commands are behaviorally equivalent if they
+evaluate to the same ending state whenever they are started in the
+same initial state," because some commands, when run in some
+starting states, don't terminate in any final state at all!
 
-  What we need instead is this: two commands are behaviorally
-  equivalent if, for any given starting state, they either (1) both
-  diverge or else (2) both terminate in the same final state.  A
-  compact way to express this is "if the first one terminates in a
-  particular state then so does the second, and vice versa."
+What we need instead is this: two commands are behaviorally
+equivalent if, for any given starting state, they either (1) both
+diverge or else (2) both terminate in the same final state.  A
+compact way to express this is "if the first one terminates in a
+particular state then so does the second, and vice versa."
 ::::
 
 ```lean
 def Com.Equiv (c₁ c₂ : Com) : Prop :=
     ∀ {st st' : State},
-      (st =[ ~c₁ ]=> st') ↔ (st =[ ~c₂ ]=> st')
+      (st =[ c₁ ]=> st') ↔ (st =[ c₂ ]=> st')
 
-theorem Com.equiv_def {c₁ c₂ : Com} : c₁.Equiv c₂ ↔
-    ∀ {st st' : State}, (st =[ ~c₁ ]=> st') ↔ (st =[ ~c₂ ]=> st') := by rfl
+instance : Equiv Com where
+  equiv := Com.Equiv
+
+@[simp]
+theorem Com.equiv_notation {c₁ c₂ : Com} : c₁.Equiv c₂ ↔ c₁ ≃ c₂ := by rfl
+@[simp]
+theorem Com.equiv_def {c₁ c₂ : Com} : c₁ ≃ c₂ ↔
+    ∀ {st st' : State}, (st =[ c₁ ]=> st') ↔ (st =[ c₂ ]=> st') := by rfl
 ```
 
 ## Simple Examples
@@ -136,11 +140,11 @@ namespace Com
 
 ::::full
   For examples of command equivalence, let's start by looking at
-  a trivial equivalence involving `skip`.
+  a trivial equivalence involving {name}`skip`.
 ::::
 
 ```lean
-theorem skip_left {c : Com} : (imp { skip; ~c }).Equiv c := by
+theorem skip_left {c : Com} : imp { skip; c } ≃ c := by
   workinclass!
     rw [equiv_def]
     intro st st''
@@ -155,11 +159,11 @@ theorem skip_left {c : Com} : (imp { skip; ~c }).Equiv c := by
 ```
 
 :::::exercise (rating := 2) (name:= "skip_right")
-Prove that adding a `skip` _after_ a command also results in an
+Prove that adding a {name}`skip` _after_ a command also results in an
 equivalent program.
 
 ```lean
-theorem skip_right {c : Com} : (imp { ~c; skip }).Equiv c := by
+theorem skip_right {c : Com} : imp { c; skip } ≃ c := by
   solution!
     rw [equiv_def]
     intro st st''
@@ -180,7 +184,7 @@ commands.
 ::::
 
 ```lean
-theorem if_true_simple {c₁ c₂ : Com} : (imp {if (true) {~c₁} else {~c₂}}).Equiv c₁ := by
+theorem if_true_simple {c₁ c₂ : Com} : imp {if (true) {c₁} else {c₂}} ≃ c₁ := by
   rw [equiv_def]
   intro st st'
   constructor
@@ -195,52 +199,47 @@ theorem if_true_simple {c₁ c₂ : Com} : (imp {if (true) {~c₁} else {~c₂}}
 
 ::::full
 Of course, no programmer would write a conditional whose condition
-is literally `true`.  (At least, no human programmer -- compilers
+is literally `true`.  (At least, no human programmer - compilers
 and macro preprocessors do this sort of thing internally all the
 time!) But they might write one whose condition is _equivalent_ to
 true:
 ::::
-:::dev "Sati (satiscugcat)"
-The to\_verso script seems to use `\[\]` blocks, but these seem to
-cause problems with the tilde. Currently skipping them and just using
-backticks.
-:::
+
 ::::full
-_Theorem_: If `b` is equivalent to `true`, then `if (~b) {~c₁}
-else {~c₂}` is equivalent to `c₁`.
+_Theorem_: If `b` is equivalent to `true`, then `if (b) {c₁} else {c₂}` is equivalent to `c₁`.
 _Proof_:
- - (`->`) We must show, for all `st` and `st'`, that if
-   `st =[ imp {if (~b) {~c₁} else {~c₂}} ]=> st'` then
+ - (`→`) We must show, for all `st` and `st'`, that if
+   `st =[ imp {if (b) {c₁} else {c₂}} ]=> st'` then
    `st =[ c₁ ]=> st'`.
 
    Proceed by cases on the rules that could possibly have been
-   used to show `st =[ imp {if (~b) {~c₁} else {~c₂}} ]=> st'`,
-   namely `Com.EvalR.ifTrue` and `Com.EvalR.ifFalse`.
+   used to show `st =[ imp {if (b) {c₁} else {c₂}} ]=> st'`,
+   namely {name}`Com.EvalR.ifTrue` and {name}`Com.EvalR.ifFalse`.
 
    - Suppose the final rule in the derivation of
-     `st =[ imp {if (~b) {~c₁} else {~c₂}} ]=> st'` was `Com.EvalR.ifTrue`.
-     We then have, by the premises of `Com.EvalR.ifTrue`, that
+     `st =[ imp {if (b) {c₁} else {c₂}} ]=> st'` was {name}`Com.EvalR.ifTrue`.
+     We then have, by the premises of {name}`Com.EvalR.ifTrue`, that
      `st =[ c₁ ]=> st'`. This is exactly what we set out to prove.
 
    - On the other hand, suppose the final rule in the derivation
-     of `st =[ imp {if (~b) {~c₁} else {~c₂}} ]=> st'` was `Com.EvalR.ifFalse`.
+     of `st =[ imp {if (b) {c₁} else {c₂}} ]=> st'` was `Com.EvalR.ifFalse`.
      We then know that `b.eval st = false` and `st =[ c₂ ]=> st'`.
 
      Recall that `b` is equivalent to `true`, i.e., forall `st`,
      `b.eval st = (bexp {true}).eval st`.  In particular, this means
      that `b.eval st = true`, since `(bexp {true}).eval st = true`.  But
-     this is a contradiction, since `Com.EvalR.ifFalse` requires that
+     this is a contradiction, since {name}`Com.EvalR.ifFalse` requires that
      `b.eval st = false`.  Thus, the final rule could not have
-     been `Com.EvalR.ifFalse`.
+     been {name}`Com.EvalR.ifFalse`.
 
  - (`<-`) We must show, for all `st` and `st'`, that if
    `st =[ c₁ ]=> st'` then
-   `st =[ imp {if (~b) {~c₁} else {~c₂}} ]=> st'`.
+   `st =[ imp {if (b) {c₁} else {c₂}} ]=> st'`.
 
    Since `b` is equivalent to `true`, we know that `b.eval st` =
    `(bexp {true}).eval st = true` = `true`.  Together with the assumption that
-   `st =[ c₁ ]=> st'`, we can apply `Com.EvalR.ifTrue` to derive
-   `st =[ imp {if (~b) {~c₁} else {~c₂}} ]=> st'`.
+   `st =[ c₁ ]=> st'`, we can apply {name}`Com.EvalR.ifTrue` to derive
+   `st =[ imp {if (b) {c₁} else {c₂}} ]=> st'`.
 ::::
 
 ::::full
@@ -248,45 +247,31 @@ Here is the formal version of this proof:
 ::::
 
 ```lean
-theorem if_true {b : Bexp} {c₁ c₂ : Com} (hb : b.Equiv (bexp {true})) :
-    (imp {if (~b) {~c₁} else {~c₂}}).Equiv c₁ := by
+theorem if_true {b : Bexp} {c₁ c₂ : Com} (hb : b ≃ bexp {true}) :
+    imp {if (b) {c₁} else {c₂}} ≃ c₁ := by
   rw [equiv_def]
-  rw [Bexp.equiv_def] at hb
   intro st st'
   constructor
   · intro h
-    inversion h with
-    | ifTrue hb' hc =>
-      exact hc
-    | ifFalse hb' hc =>
-      rw [hb] at hb'
-      simp at hb'
+    inversion h <;> simp_all
   · intro h
     apply EvalR.ifTrue _ h
-    rw [hb]
-    simp
+    simp_all
 ```
 
 :::::exercise (rating := 2) (name := "if_false_equiv")
 ```lean
-theorem if_false {b : Bexp} {c₁ c₂ : Com} (hb : b.Equiv (bexp {false})) :
-    (imp {if (~b) {~c₁} else {~c₂}}).Equiv c₂ := by
+theorem if_false {b : Bexp} {c₁ c₂ : Com} (hb : b ≃ bexp {false}) :
+    imp {if (b) {c₁} else {c₂}} ≃ c₂ := by
   solution!
     rw [equiv_def]
-    rw [Bexp.equiv_def] at hb
     intro st st'
     constructor
     · intro h
-      inversion h with
-      | ifTrue hb' hc =>
-        rw [hb] at hb'
-        simp at hb'
-      | ifFalse hb' hc =>
-        exact hc
+      inversion h <;> simp_all
     · intro h
       apply EvalR.ifFalse _ h
-      rw [hb]
-      simp
+      simp_all
 ```
 :::::
 
@@ -297,8 +282,8 @@ condition.
 
 ```lean
 theorem swap_if_branches {b : Bexp} {c₁ c₂ : Com} :
-    (imp {if (~b) {~c₁} else {~c₂}}).Equiv
-    (imp {if (¬ ~b) {~c₂} else {~c₁}}) := by
+    imp {if (b) {c₁} else {c₂}} ≃
+    imp {if (¬ b) {c₂} else {c₁}} := by
   solution!
     rw [equiv_def]
     intro st st'
@@ -324,9 +309,9 @@ theorem swap_if_branches {b : Bexp} {c₁ c₂ : Com} :
 
 ::::full
 For `while` loops, we can give a similar pair of theorems.  A loop
-whose guard is equivalent to `false` is equivalent to `skip`,
-while a loop whose guard is equivalent to `true` is equivalent to
-`while (true) {skip;} end` (or any other non-terminating program).
+whose guard is equivalent to {name}`false` is equivalent to {name}`skip`,
+while a loop whose guard is equivalent to {name}`true` is equivalent to
+`while (true) {skip} end` (or any other non-terminating program).
 ::::
 
 ::::full
@@ -334,22 +319,20 @@ The first of these facts is easy.
 ::::
 
 ```lean
-theorem while_false_equiv {b : Bexp} {c : Com} (hb : b.Equiv (bexp {false})) :
-    (imp {while (~b) {~c}}).Equiv
-    (imp {skip}) := by
+theorem while_false_equiv {b : Bexp} {c : Com} (hb : b ≃ bexp {false}) :
+    imp {while (b) {c}} ≃ imp {skip} := by
   rw [equiv_def]
-  rw [Bexp.equiv_def] at hb
   intro st st''
   constructor
   · intro h
     inversion h with
     | whileFalse => exact EvalR.skip
     | whileTrue st' hb' hc hloop =>
-      simp [hb] at hb'
+      simp_all
   · intro h
     inversion h
     apply EvalR.whileFalse
-    simp [hb]
+    simp_all
 ```
 
 :::::exercise (rating := 2) (name := "while_false_informal") (level:= Advanced) (manual:= true)
@@ -358,65 +341,64 @@ Write an informal proof of `while_false_equiv`.
 
 ::::full
 To prove the second fact, we need an auxiliary lemma stating that
-`while` loops whose guards are equivalent to `true` never
+`while` loops whose guards are equivalent to {name}`true` never
 terminate.
 ::::
 
 ::::full
-_Lemma_: If `b` is equivalent to `true`, then it cannot be
-the case that `st =[ while (~b) {~c} ]=> st'`.
+_Lemma_: If `b` is equivalent to {name}`true`, then it cannot be
+the case that `st =[ while (b) {c} ]=> st'`.
 
-_Proof_: Suppose that `st =[ while (~b) {~c} ]=> st'`.  We show,
-by induction on a derivation of `st =[ while (~b) {~c} ]=> st'`,
+_Proof_: Suppose that `st =[ while (b) {c} ]=> st'`.  We show,
+by induction on a derivation of `st =[ while (b) {c} ]=> st'`,
 that this assumption leads to a contradiction. The only two cases
-to consider are `Com.EvalR.whileFalse` and `Com.EvalR.whileTrue`; the others
+to consider are {name}`Com.EvalR.whileFalse` and {name}`Com.EvalR.whileTrue`; the others
 are contradictory.
 
-- Suppose `st =[ while (~b) {~c} ]=> st'` is proved using rule
-  `Com.EvalR.whileFalse`.  Then by assumption `b.eval st = false`. But
+- Suppose `st =[ while (b) {c} ]=> st'` is proved using rule
+  {name}`Com.EvalR.whileFalse`.  Then by assumption `b.eval st = false`. But
   this contradicts the assumption that `b` is equivalent to
   `true`.
 
-- Suppose `st =[ while (~b) {~c} ]=> st'` is proved using rule
-  `Com.EvalR.whileTrue`.  We must have:
+- Suppose `st =[ while (b) {c} ]=> st'` is proved using rule
+  {name}`Com.EvalR.whileTrue`.  We must have:
 
   1. `b.eval st = true`, and
   2. there is some `st₀` such that `st =[ c ] => st₀` and
-     `st₀ =[ while (~b) {~c} ]=> st'`.
+     `st₀ =[ while (b) {c} ]=> st'`.
   3. Also, we are given an induction hypothesis saying that
-     `st₀ =[ while (~b) {~c} ]=> st'` leads to a contradiction,
+     `st₀ =[ while (b) {c} ]=> st'` leads to a contradiction,
 
   We obtain a contradiction by 2 and 3.
 ::::
 
 ```lean
-theorem while_true_nonterm {b : Bexp} {c : Com} {st st' : State} (hb : b.Equiv (bexp {true})) :
-    ¬ st =[ while (~b) {~c} ]=> st' := by
+theorem while_true_nonterm {b : Bexp} {c : Com} {st st' : State} (hb : b ≃ bexp {true}) :
+    ¬ st =[ while (b) {c} ]=> st' := by
   workinclass!
     intro contra
-    generalize heq : (imp {while (~b) {~c}}) = com at contra
+    generalize heq : (imp {while (b) {c}}) = com at contra
     induction contra with
-    | @whileFalse b' s0 c0 hb' =>
+    | whileFalse hb' =>
       injection heq with hbeq hceq
       subst hbeq
-      rw [Bexp.equiv_def] at hb
-      simp [hb] at hb'
-    | @whileTrue s0 s0' s0'' b' c0 hb' hc' hwhile ih1 ih2 =>
+      simp_all -- hb and hb' are contradictory
+    | whileTrue hb' hc' hwhile ih1 ih2 =>
       exact ih2 heq
     | skip | asgn | seq | ifTrue | ifFalse =>
-      contradiction -- heq says that different commands are equal
+      contradiction -- `heq` says that different commands are equal
 ```
 :::::exercise (rating := 2) (name := "while_true_nonterm_informal") (manual:= true)
 Explain what the lemma `while_true_nonterm` means in English.
 :::::
+
 :::::exercise (rating := 2) (name := "while_true")
-Prove the following theorem. _Hint_: You'll want to use
-`while_true_nonterm` here.
+Prove the following theorem.
+_Hint_: You'll want to use `while_true_nonterm` here.
 
 ```lean
-theorem while_true {b : Bexp} {c : Com} (hb : b.Equiv (bexp {true})) :
-    (imp {while (~b) {~c}}).Equiv
-    (imp {while (true) {skip}}) := by
+theorem while_true {b : Bexp} {c : Com} (hb : b ≃ bexp {true}) :
+    imp {while (b) {c}} ≃ imp {while (true) {skip}} := by
   solution!
     rw [equiv_def]
     intro st st'
@@ -444,11 +426,11 @@ interest!
 
 ```lean
 theorem loop_unrolling {b : Bexp} {c : Com} :
-    (imp {while (~b) {~c}}).Equiv
-    (imp {
-      if (~b) {~c} else {skip};
-      while (~b) {~c}
-    }) := by
+    imp { while (b) {c} } ≃
+    imp {
+      if (b) {c} else {skip};
+      while (b) {c}
+    } := by
   workinclass!
     rw [equiv_def]
     intro st st'
@@ -472,9 +454,28 @@ theorem loop_unrolling {b : Bexp} {c : Com} :
           inversion hc
           exact h2
 ```
-:::dev "Sati (satiscugcat)"
-Leaving out optional exercise `seq_assoc` for now.
-:::
+
+:::::full
+::::exercise (rating := 2) (name := "seq_assoc") (optional:= true)
+```lean
+theorem seq_assoc {c₁ c₂ c₃ : Com} :
+  imp {~(imp {c₁; c₂}); c₃} ≃ imp {c₁; c₂; c₃} := by
+    solution!
+      intro st₁ st₂
+      constructor <;> intro h
+      · inversion h with
+        | seq h₁ h₂ =>
+            inversion h₁
+            apply EvalR.seq; assumption
+            apply EvalR.seq <;> assumption
+      · inversion h with
+        | seq h₁ h₂ =>
+            inversion h₂
+            apply EvalR.seq <;> try assumption
+            apply EvalR.seq <;> assumption
+```
+::::
+:::::
 
 ::::full
 Proving program properties involving assignments is one place
@@ -485,8 +486,7 @@ in handy.
 
 ```lean
 theorem identity_assignment {X : Ident} :
-    (imp {X := X}).Equiv
-    (imp {skip}) := by
+    imp { X := X } ≃ imp { skip } := by
   rw [equiv_def]
   intro st st'
   constructor
@@ -498,18 +498,16 @@ theorem identity_assignment {X : Ident} :
       exact Com.EvalR.skip
   · intro h
     inversion h
-    suffices st =[ X := X ]=> X →ₜ st[X] ; st by
-      simp only [TotalMap.update_same] at this
-      exact this
-    apply Com.EvalR.asgn
-    simp
+    have h' : st =[ X := X ]=> X →ₜ st[X] ; st := by
+      apply Com.EvalR.asgn
+      simp
+    simp_all [TotalMap.update_same]
 ```
 
 :::::exercise (rating := 2) (name := "assign_equiv")
 ```lean
-theorem assign_equiv {X : Ident} {a : Aexp} (ha : Aexp.Equiv (aexp {X}) a) :
-    (imp {skip}).Equiv
-    (imp {X := ~a}) := by
+theorem assign_equiv {X : Ident} {a : Aexp} (ha : aexp { X } ≃ a) :
+    imp { skip } ≃ imp { X := a } := by
   solution!
     rw [equiv_def]
     rw [Aexp.equiv_def] at ha
@@ -517,11 +515,10 @@ theorem assign_equiv {X : Ident} {a : Aexp} (ha : Aexp.Equiv (aexp {X}) a) :
     constructor
     · intro h
       inversion h
-      suffices st =[ X := ~a ]=> X →ₜ st[X]; st by
-        simp only [TotalMap.update_same] at this
-        exact this
-      apply Com.EvalR.asgn
-      simp [← ha]
+      have h' : st =[ X := ~a ]=> X →ₜ st[X]; st := by
+        apply Com.EvalR.asgn
+        simp [← ha]
+      simp_all [← ha]
     · intro h
       inversion h with
       | asgn n h =>
@@ -531,9 +528,95 @@ theorem assign_equiv {X : Ident} {a : Aexp} (ha : Aexp.Equiv (aexp {X}) a) :
 ```
 :::::
 
-:::dev "Sati (satiscugcat)"
-Leaving out optional exercise `equiv_classes` for now.
-:::
+:::::full
+::::exercise (rating := 2) (name := "equiv_classes") (manual:= true) (optional := true)
+Given the following programs, group together those that are
+equivalent in Imp. Your answer should be given as a list of lists,
+where each sub-list represents a group of equivalent programs. For
+example, if you think programs (a) through (h) are all equivalent
+to each other, but not to (i), your answer should look like this:
+
+```
+[ [progA, progB, progC, progD, progE, progF, progG, progH], [progI] ]
+```
+
+Write down your answer below in the definition of  `equiv_classes`
+
+```lean
+def progA : Com :=
+  imp {
+    while (X > 0) {
+       X := X + 1
+    }
+  }
+
+def progB : Com :=
+  imp {
+    if (X = 0) {
+       X := X + 1;
+       Y := 1
+     } else {
+       Y := 0
+     };
+     X := X - Y;
+     Y := 0
+  }
+
+def progC : Com :=
+  imp { skip }
+
+def progD : Com :=
+  imp {
+    while (X ≠ 0) {
+       X := (X * Y) + 1
+    }
+  }
+
+def progE : Com :=
+  imp { Y := 0 }
+
+def progF : Com :=
+  imp {
+    Y := X + 1;
+    while (X ≠ Y) {
+      Y := X + 1
+    }
+  }
+
+def progG : Com :=
+  imp {
+    while (true) {
+      skip
+    }
+  }
+
+def progH : Com :=
+  imp {
+    while (X ≠ X) {
+      X := X + 1
+    }
+  }
+
+def progI : Com :=
+  imp {
+    while (X ≠ Y) {
+      X := Y + 1
+    }
+  }
+```
+
+```lean
+def equiv_classes : List (List Com) :=
+-- SOLUTION
+  [ [progA, progD] ,
+    [progB, progE] ,
+    [progC, progH] ,
+    [progF, progG] ,
+    [progI] ]
+-- END SOLUTION
+```
+::::
+:::::
 
 # Properties of Behavior Equivalence
 
@@ -544,80 +627,39 @@ We next consider some fundamental properties of program equivalence.
 ## Behavioral Equivalence is an Equivalence
 
 ::::full
-First, let's verify that the equivalences on `Aexp`s, `Bexp`s, and
-`Com`s really are _equivalences_ -- ie, that they are reflexive,
+First, let's verify that the equivalences on {name}`Aexp`s, {name}`Bexp`s, and
+{name}`Com`s really are _equivalences_ - ie, that they are reflexive,
 symmetric, and transitive. These proofs are all easy.
 ::::
 
 ```lean
 end Com
 
-theorem Aexp.equiv_refl (a : Aexp) : a.Equiv a := by
-  rw [equiv_def]
-  intro st
-  rfl
+theorem Aexp.equiv_refl (a : Aexp) : a ≃ a := by simp_all
+theorem Aexp.equiv_symm {a₁ a₂ : Aexp} (h : a₁ ≃ a₂) : a₂ ≃ a₁ := by simp_all
+theorem Aexp.equiv_trans {a₁ a₂ a₃ : Aexp} (h₁ : a₁ ≃ a₂) (h₂ : a₂ ≃ a₃) : a₁ ≃ a₃ := by simp_all
+
+theorem Bexp.equiv_refl {b : Bexp} : b ≃ b := by simp_all
+theorem Bexp.equiv_symm {b₁ b₂ : Bexp} (h : b₁ ≃ b₂) : b₂ ≃ b₁ := by simp_all
+theorem Bexp.equiv_trans {b₁ b₂ b₃ : Bexp} (h₁ : b₁ ≃ b₂) (h₂ : b₂ ≃ b₃) : b₁ ≃ b₃ := by simp_all
+
+theorem Com.equiv_refl {c : Com} : c ≃ c := by simp_all
+theorem Com.equiv_symm {c₁ c₂ : Com} (h : c₁ ≃ c₂) : c₂ ≃ c₁ := by simp_all
+theorem Com.equiv_trans {c₁ c₂ c₃ : Com} (h₁ : c₁ ≃ c₂) (h₂ : c₂ ≃ c₃) : c₁ ≃ c₃ := by simp_all
 ```
+
+::::full
+Lean has a standard library definition for relations that are equivalences, unsurprisingly called
+{name}`Equivalence`. To show that a relation is an {name}`Equivalence`,
+one needs only supply proofs of the three properties above:
 
 ```lean
-theorem Aexp.equiv_symm {a₁ a₂ : Aexp} (h : a₁.Equiv a₂) : a₂.Equiv a₁ := by
-  rw [equiv_def] at h ⊢
-  intro st
-  rw [h]
+theorem Com.equiv_equivalence : Equivalence Com.Equiv where
+  refl := @Com.equiv_refl
+  symm := Com.equiv_symm
+  trans := Com.equiv_trans
 ```
-
-```lean
-theorem Aexp.equiv_trans {a₁ a₂ a₃ : Aexp} (h₁ : a₁.Equiv a₂) (h₂ : a₂.Equiv a₃) :
-    a₁.Equiv a₃ := by
-  rw [equiv_def] at h₁ h₂ ⊢
-  intro st
-  rw [h₁, h₂]
-```
-
-
-```lean
-theorem Bexp.equiv_refl {b : Bexp} : b.Equiv b := by
-  rw [equiv_def]
-  intro st
-  rfl
-```
-
-```lean
-theorem Bexp.equiv_symm {b₁ b₂ : Bexp} (h : b₁.Equiv b₂) : b₂.Equiv b₁ := by
-  rw [equiv_def]
-  intro st
-  rw [h]
-```
-
-```lean
-theorem Bexp.equiv_trans {b₁ b₂ b₃ : Bexp} (h₁ : b₁.Equiv b₂) (h₂ : b₂.Equiv b₃) :
-    b₁.Equiv b₃ := by
-  rw [equiv_def]
-  intro st
-  rw [h₁, h₂]
-```
-
-
-```lean
-theorem Com.equiv_refl {c : Com} : c.Equiv c := by
-  rewrite [equiv_def]
-  intro st st'
-  rfl
-```
-
-```lean
-theorem Com.equiv_symm {c₁ c₂ : Com} (h : c₁.Equiv c₂) : c₂.Equiv c₁ := by
-  rw [equiv_def] at h ⊢
-  intro st st'
-  rw [h]
-```
-
-```lean
-theorem Com.equiv_trans {c₁ c₂ c₃ : Com} (h₁ : c₁.Equiv c₂) (h₂ : c₂.Equiv c₃) :
-    c₁.Equiv c₃ := by
-  rw [equiv_def] at h₁ h₂ ⊢
-  intro st st'
-  rw [h₁, h₂]
-```
+::::
 
 ## Behavioral Equivalence is a Congruence
 
@@ -627,14 +669,14 @@ Less obviously, behavioral equivalence is also a _congruence_.
 That is, the equivalence of two subprograms implies the
 equivalence of the larger programs in which they are embedded:
 
-             aequiv a a'
+              a ≃ a'
      -------------------------
-     cequiv (x := a) (x := a')
+        (x := a) ≃ (x := a')
 
-          cequiv c1 c1'
-          cequiv c2 c2'
+            c1 ≃ c1'
+            c2 ≃ c2'
      --------------------------
-     cequiv (c1;c2) (c1';c2')
+      (c1 ; c2) ≃ (c1' ; c2')
 
 ... and so on for the other forms of commands.
 
@@ -651,16 +693,15 @@ properties are important in the following section (in the proof of
 us to replace a small part of a large program with an equivalent
 small part and know that the whole large programs are equivalent
 _without_ doing an explicit proof about the parts that didn't
-change -- i.e., the "proof burden" of a small change to a large
+change - i.e., the "proof burden" of a small change to a large
 program is proportional to the size of the change, not the
 program!
 ::::
 
 
 ```lean
-theorem Com.congruence.asgn {x : Ident} {a a' : Aexp} (ha : a.Equiv a') :
-    (imp {x := ~a}).Equiv
-    (imp {x := ~a'}) := by
+theorem Com.congruence.asgn {x : Ident} {a a' : Aexp} (ha : a ≃ a') :
+    imp {x := a} ≃ imp {x := a'} := by
   rw [equiv_def]
   intro st st'
   constructor <;>
@@ -669,8 +710,7 @@ theorem Com.congruence.asgn {x : Ident} {a a' : Aexp} (ha : a.Equiv a') :
     | asgn n h =>
       subst h
       apply Com.EvalR.asgn
-      rw [Aexp.equiv_def] at ha
-      rw [ha]
+      simp_all
 ```
 
 ::::full
@@ -679,38 +719,39 @@ since it requires induction.
 
 _Theorem_: Equivalence is a congruence for `while` -- that is, if
 `b` is equivalent to `b'` and `c` is equivalent to `c'`, then
-`while (~b) {~c}` is equivalent to `while (~b') {~c'}`.
+`while (b) {c}` is equivalent to `while (b') {c'}`.
 
 _Proof_: Suppose `b` is equivalent to `b'` and `c` is
 equivalent to `c'`.  We must show, for every `st` and `st'`, that
-`st =[ while (~b) {~c} ]=> st'` iff `st = while (~b') {~c'}
-]=> st'`.  We consider the two directions separately.
+`st =[ while (b) {c} ]=> st'` iff `st = while (b') {c'}]=> st'`.
+We consider the two directions separately.
 
-  - (`->`) We show that `st =[ while (~b) {~c} ]=> st'` implies
-    `st =[ while (~b') {~c'} ]=> st'`, by induction on a
-    derivation of `st =[ while (~b) {~c} ]=> st'`.  The only
+  - (`→`) We show that `st =[ while (b) {c} ]=> st'` implies
+    `st =[ while (b') {c'} ]=> st'`, by induction on a
+    derivation of `st =[ while (b) {c} ]=> st'`.  The only
     nontrivial cases are when the final rule in the derivation is
-    `Com.EvalR.whileFalse` or `Com.EvalR.whileTrue`.
+    {name}`Com.EvalR.whileFalse` or {name}`Com.EvalR.whileTrue`.
 
-      - `Com.EvalR.whileFalse`: In this case, the form of the rule gives us
-        `beval st b = false` and `st = st'`.  But then, since
-        `b` and `b'` are equivalent, we have `beval st b' =false`,
-        and `Com.EvalR.whileFalse` applies, giving us
-        `st =[ while (~b') {~c'} ]=> st'`, as required.
+      - {name}`Com.EvalR.whileFalse`: In this case, the form of the rule gives us
+        `b.eval st = false` and `st = st'`.  But then, since
+        `b` and `b'` are equivalent, we have `b'.eval st = false`,
+        and {name}`Com.EvalR.whileFalse` applies, giving us
+        `st =[ while (b') {c'} ]=> st'`, as required.
 
-      - `Com.EvalR.whileTrue`: The form of the rule now gives us `beval st b = true`,
-        with `st =[ c ]=> st'0` and `st'0 =[ while {~b} {~c} ]=> st'`
-        for some state `st'0`, with the
-        induction hypothesis `st'0 =[ while (~b') {~c'} ]=> st'`.
+      - {name}`Com.EvalR.whileTrue`: The form of the rule now gives us `b.eval st = true`,
+        with `st =[ c ]=> st'₀` and `st'₀ =[ while {b} {c} ]=> st'`
+        for some state `st'₀`, with the
+        induction hypothesis `st'₀ =[ while (b') {c'} ]=> st'`.
 
         Since `c` and `c'` are equivalent, we know that `st =[ c']=> st'0`.
         And since `b` and `b'` are equivalent,
-        we have `beval st b' = true`.  Now `Com.EvalR.whileTrue` applies,
-        giving us `st =[ while (~b') {~c'} ]=> st'`, as
+        we have `b'.eval st = true`.  Now {name}`Com.EvalR.whileTrue` applies,
+        giving us `st =[ while (b') {c'} ]=> st'`, as
         required.
 
-  - (`<-`) Similar.
+  - (`←`) Similar.
 ::::
+
 :::dev "Sati (satiscugcat)"
 ```
 NOT PORTED YET - remaining portions of Equiv.v left (apart from the portions explicitly stated so far).
